MESI: still trying to prove [InvWB] (changed the invariant statement) (heads-up: not compilable)

src/Ex/Mesi/MesiInvInv1.v
@@ -31,13 +31,18 @@ Proof.
   discriminate.
 Qed.
 
-(* Definition NoRsSI (oidx: IdxT) (msgs: MessagePool Msg) := *)
-(*   MsgsNotExist [(downTo oidx, (MRs, mesiInvRs)); *)
-(*                   (downTo oidx, (MRs, mesiRsS))] msgs. *)
+Definition NoRsME (oidx: IdxT) (msgs: MessagePool Msg) :=
+  MsgsNotExist [(downTo oidx, (MRs, mesiRsM));
+                  (downTo oidx, (MRs, mesiRsE))] msgs.
+
+Definition NoRsSI (oidx: IdxT) (msgs: MessagePool Msg) :=
+  MsgsNotExist [(downTo oidx, (MRs, mesiRsS));
+                  (downTo oidx, (MRs, mesiInvRs))] msgs.
 
 Definition ObjInS (ost: OState) :=
-  (ost#[dir].(dir_st) <= mesiS -> mesiS <= ost#[status]) /\
-  (ost#[dir].(dir_st) <= mesiE -> ost#[owned] = true).
+  ost#[dir].(dir_st) <= mesiS ->
+  (ost#[status] = mesiS /\ ost#[owned] = true) \/
+  mesiE <= ost#[status].
 
 Definition InvDirME (topo: DTree) (st: MState): Prop :=
   forall oidx pidx,
@@ -46,8 +51,9 @@ Definition InvDirME (topo: DTree) (st: MState): Prop :=
       orq <+- (bst_orqs st)@[oidx];
       post <+- (bst_oss st)@[pidx];
       porq <+- (bst_orqs st)@[pidx];
-      (ObjDirME porq post oidx -> orq@[upRq] = None ->
-       NoRsI oidx (bst_msgs st) /\ ObjInS ost).
+      (ObjDirME porq post oidx ->
+       NoRsME oidx (bst_msgs st) ->
+       (NoRsSI oidx (bst_msgs st) /\ ObjInS ost)).
 
 Section InvDirME.
   Variable (tr: tree).
@@ -94,19 +100,21 @@ Section InvDirME.
     destruct (orqs@[oidx]) as [orq|] eqn:Horq; simpl in *; auto.
     destruct (oss@[pidx]) as [post|] eqn:Hpost; simpl in *; auto.
     destruct (orqs@[pidx]) as [porq|] eqn:Hporq; simpl in *; auto.
-    intros; specialize (H H3 H4); dest.
-    split; [|assumption].
-    apply MsgsP_other_midx_enqMsgs; [assumption|].
-    destruct H1; simpl.
-    eapply DisjList_SubList; [eassumption|].
-    eapply DisjList_comm, DisjList_SubList.
-    - eapply SubList_trans;
-        [|eapply tree2Topo_obj_chns_minds_SubList with (oidx:= oidx)].
-      + solve_SubList.
-      + specialize (H0 oidx); simpl in H0.
-        rewrite Host in H0; simpl in H0.
-        eassumption.
-    - apply tree2Topo_minds_merqs_disj.
+    intros.
+    (* intros; specialize (H H3 H4); dest. *)
+    (* split; [|assumption]. *)
+    (* apply MsgsP_other_midx_enqMsgs; [assumption|]. *)
+    (* destruct H1; simpl. *)
+    (* eapply DisjList_SubList; [eassumption|]. *)
+    (* eapply DisjList_comm, DisjList_SubList. *)
+    (* - eapply SubList_trans; *)
+    (*     [|eapply tree2Topo_obj_chns_minds_SubList with (oidx:= oidx)]. *)
+    (*   + solve_SubList. *)
+    (*   + specialize (H0 oidx); simpl in H0. *)
+    (*     rewrite Host in H0; simpl in H0. *)
+    (*     eassumption. *)
+    (* - apply tree2Topo_minds_merqs_disj. *)
+    admit.
   Qed.
 
   Lemma mesi_InvDirME_ext_out:
@@ -124,35 +132,39 @@ Section InvDirME.
     destruct (orqs@[oidx]) as [orq|] eqn:Horq; simpl in *; auto.
     destruct (oss@[pidx]) as [post|] eqn:Hpost; simpl in *; auto.
     destruct (orqs@[pidx]) as [porq|] eqn:Hporq; simpl in *; auto.
-    intros; specialize (H H2 H3); dest.
-    split; [|assumption].
-    apply MsgsP_deqMsgs; assumption.
+    (* intros; specialize (H H2 H3); dest. *)
+    (* split; [|assumption]. *)
+    (* apply MsgsP_deqMsgs; assumption. *)
+    admit.
   Qed.
 
-  Lemma InvDirME_other_msg_id_enqMP:
+  Lemma InvDirME_enqMP:
     forall oss orqs msgs,
       InvDirME topo {| bst_oss:= oss; bst_orqs:= orqs; bst_msgs:= msgs |} ->
       forall midx msg,
         msg.(msg_id) <> mesiInvRs ->
+        msg.(msg_id) <> mesiRsS ->
         InvDirME topo {| bst_oss:= oss; bst_orqs:= orqs;
                          bst_msgs:= enqMP midx msg msgs |}.
   Proof.
     red; simpl; intros.
-    specialize (H _ _ H1); simpl in H.
+    specialize (H _ _ H2); simpl in H.
     destruct (oss@[oidx]) as [ost|] eqn:Host; simpl in *; auto.
     destruct (orqs@[oidx]) as [orq|] eqn:Horq; simpl in *; auto.
     destruct (oss@[pidx]) as [post|] eqn:Hpost; simpl in *; auto.
     destruct (orqs@[pidx]) as [porq|] eqn:Hporq; simpl in *; auto.
     intros.
-    specialize (H H2 H3); dest.
+    apply MsgsP_enqMP_inv in H4.
+    specialize (H H3 H4); dest.
     split; [|assumption].
     apply MsgsP_other_msg_id_enqMP.
     - apply H; auto.
     - simpl; intro Hx.
       destruct Hx; auto.
+      destruct H6; auto.
   Qed.
   
-  Lemma InvDirME_other_msg_id_enqMsgs:
+  Lemma InvDirME_enqMsgs:
     forall oss orqs msgs,
       InvDirME topo {| bst_oss:= oss; bst_orqs:= orqs; bst_msgs:= msgs |} ->
       forall nmsgs,
@@ -166,23 +178,28 @@ Section InvDirME.
     induction nmsgs as [|[nmidx nmsg] nmsgs]; simpl; intros; auto.
     inv H0; dest.
     apply IHnmsgs; auto.
-    apply InvDirME_other_msg_id_enqMP; assumption.
+    apply InvDirME_enqMP; assumption.
   Qed.
 
   Lemma InvDirME_deqMP:
     forall oss orqs msgs,
       InvDirME topo {| bst_oss:= oss; bst_orqs:= orqs; bst_msgs:= msgs |} ->
-      forall midx,
+      forall midx msg,
+        FirstMP msgs midx msg ->
+        msg.(msg_id) <> mesiRsM ->
+        msg.(msg_id) <> mesiRsE ->
         InvDirME topo {| bst_oss:= oss; bst_orqs:= orqs;
                          bst_msgs:= deqMP midx msgs |}.
   Proof.
     unfold InvDirME; simpl; intros.
-    specialize (H _ _ H0).
+    specialize (H _ _ H3).
     destruct (oss@[oidx]) as [ost|] eqn:Host; simpl in *; auto.
     destruct (orqs@[oidx]) as [orq|] eqn:Horq; simpl in *; auto.
     destruct (oss@[pidx]) as [post|] eqn:Hpost; simpl in *; auto.
     destruct (orqs@[pidx]) as [porq|] eqn:Hporq; simpl in *; auto.
-    intros; specialize (H H1 H2); dest.
+    intros.
+    eapply MsgsP_other_msg_id_deqMP_inv in H5; [|eassumption|simpl; intro; intuition].
+    specialize (H H4 H5); dest.
     split; [|assumption].
     apply MsgsP_deqMP; assumption.
   Qed.
@@ -190,41 +207,66 @@ Section InvDirME.
   Lemma InvDirME_deqMsgs:
     forall oss orqs msgs,
       InvDirME topo {| bst_oss:= oss; bst_orqs:= orqs; bst_msgs:= msgs |} ->
-      forall minds,
+      forall rmsgs,
+        Forall (FirstMPI msgs) rmsgs ->
+        NoDup (idsOf rmsgs) ->
+        Forall (fun idm => (valOf idm).(msg_id) <> mesiRsM /\
+                           (valOf idm).(msg_id) <> mesiRsE) rmsgs ->
         InvDirME topo {| bst_oss:= oss; bst_orqs:= orqs;
-                      bst_msgs:= deqMsgs minds msgs |}.
+                         bst_msgs:= deqMsgs (idsOf rmsgs) msgs |}.
   Proof.
     unfold InvDirME; simpl; intros.
-    specialize (H _ _ H0).
+    specialize (H _ _ H3).
     destruct (oss@[oidx]) as [ost|] eqn:Host; simpl in *; auto.
     destruct (orqs@[oidx]) as [orq|] eqn:Horq; simpl in *; auto.
     destruct (oss@[pidx]) as [post|] eqn:Hpost; simpl in *; auto.
     destruct (orqs@[pidx]) as [porq|] eqn:Hporq; simpl in *; auto.
-    intros; specialize (H H1 H2); dest.
-    split; [|assumption].
-    apply MsgsP_deqMsgs; assumption.
+    intros.
+    eapply MsgsP_other_msg_id_deqMsgs_inv in H5; try eassumption.
+    - specialize (H H4 H5); dest.
+      split; [|assumption].
+      apply MsgsP_deqMsgs; assumption.
+    - simpl.
+      apply (DisjList_spec_1 idx_dec); intros.
+      apply in_map_iff in H6; destruct H6 as [idm [? ?]].
+      rewrite Forall_forall in H2; specialize (H2 _ H7); dest; subst.
+      intro; dest_in; auto.
   Qed.
 
-  Ltac simpl_InvDirME_msgs_enqMP :=
+  Ltac solve_InvDirME_msg :=
     simpl;
     try match goal with
         | [H: msg_id ?rmsg = _ |- msg_id ?rmsg <> _] => rewrite H
         end;
     discriminate.
 
-  Ltac simpl_InvDirME_msgs_enqMsgs :=
+  Ltac solve_InvDirME_enqMsgs :=
     let idm := fresh "idm" in
     let Hin := fresh "H" in
     apply Forall_forall; intros idm Hin;
     apply in_map_iff in Hin; dest; subst;
-    split; simpl_InvDirME_msgs_enqMP.
+    split; solve_InvDirME_msg.
 
+  Ltac solve_InvDirME_deqMsgs_NoDup :=
+    match goal with
+    | [H: ValidMsgsIn _ ?msgs |- NoDup (idsOf ?msgs)] => apply H
+    end.
+
+  Ltac solve_InvDirME_deqMsgs_msg_id :=
+    match goal with
+    | [H: Forall (fun _ => msg_id _ = _) ?msgs |- Forall _ ?msgs] =>
+      eapply Forall_impl; [|eapply H];
+      simpl; intros; split; solve_InvDirME_msg
+    end.
+  
   Ltac simpl_InvDirME_msgs :=
     repeat
-      (first [apply InvDirME_other_msg_id_enqMP; [|simpl_InvDirME_msgs_enqMP..]
-             |apply InvDirME_other_msg_id_enqMsgs; [|simpl_InvDirME_msgs_enqMsgs]
-             |apply InvDirME_deqMP
-             |apply InvDirME_deqMsgs
+      (first [apply InvDirME_enqMP; [|solve_InvDirME_msg..]
+             |apply InvDirME_enqMsgs; [|solve_InvDirME_enqMsgs]
+             |eapply InvDirME_deqMP; [|eassumption|solve_InvDirME_msg..]
+             |apply InvDirME_deqMsgs; [|eassumption
+                                       |solve_InvDirME_deqMsgs_NoDup
+                                       |solve_InvDirME_deqMsgs_msg_id]
              |assumption]).
 
   Ltac disc_bind_true :=
@@ -239,7 +281,7 @@ Section InvDirME.
                destruct ov as [v|] eqn:Hov; simpl in *; [|auto]]
       end.
 
-  Ltac disc_InvDirME :=
+  Ltac disc_InvDirME_pre :=
     repeat
       match goal with
       | [Hi: InvDirME _ _ |- InvDirME _ _] =>
@@ -252,30 +294,38 @@ Section InvDirME.
       | |- _ -> _ => intros
       | [Hi: ObjDirME _ _ _ -> _, Ho: ObjDirME _ _ _ |- _] =>
         specialize (Hi Ho); dest
-      | [Hi: ?orqs@[upRq] = ?ov -> _, Ho: ?orqs@[upRq] = ?ov |- _] =>
-        specialize (Hi Ho); dest
+      | [Hi: NoRsME _ _ -> _, Hm: NoRsME _ _ |- _] =>
+        specialize (Hi Hm); dest
       | [H: ?t = ?t -> _ |- _] => specialize (H eq_refl); dest
       end.
 
-  Ltac solve_InvDirME_NoRsI_by_silent :=
+  Ltac disc_NoRsME :=
+    repeat
+      match goal with
+      | [H: NoRsME _ _ |- _] => disc_MsgsP H
+      | [Hi: NoRsME _ ?msgs -> _ /\ _,  Hm: MsgsP _ ?msgs |- _] =>
+        specialize (Hi Hm); dest
+      end.
+
+  Ltac disc_InvDirME :=
+    disc_InvDirME_pre; disc_NoRsME.
+
+  Ltac solve_InvDirME_NoRsSI_by_silent :=
     intros;
     solve_MsgsP;
     match goal with
-    | [H: _ -> NoRsI _ _ |- _] => apply H; auto; fail
+    | [H: _ -> NoRsSI _ _ |- _] => apply H; auto; fail
     end.
 
   Ltac solve_InvDirME_ObjInS_valid :=
     try assumption;
-    try match goal with
-        | |- ObjInS _ =>
-          red; simpl; split; intros; solve [reflexivity|solve_mesi]
-        end;
-    try match goal with
-        | [Ho: ObjInS _ |- ObjInS _] =>
-          let Hd := fresh "H" in
-          red; simpl; split; intros;
-          solve [solve_mesi|apply Ho; simpl; solve_mesi]
-        end.
+    try
+      match goal with
+      | Ho:ObjInS _ |- ObjInS _ =>
+        red in Ho; red; simpl in *;
+        solve [intuition solve_mesi|
+               intros; apply Ho; intuition solve_mesi]
+      end.
 
   Ltac disc_ObjDirME :=
     match goal with
@@ -283,13 +333,15 @@ Section InvDirME.
       red in H; simpl in H; dest; subst
     end.
 
-  Ltac solve_InvDirME_by_upRq_false oidx :=
+  Ltac solve_InvDirME_by_NoRsME_false :=
     exfalso;
-    disc_MsgConflictsInv oidx;
     match goal with
-    | [Hmcf: RqUpConflicts oidx _ ?msgs,
-             Hfmp:FirstMPI ?msgs (?midx, ?msg) |- _] =>
-      specialize (Hmcf (midx, msg) eq_refl (FirstMP_InMP Hfmp)); dest; auto
+    | [Hn: NoRsME _ (enqMP ?midx ?msg ?msgs) |- _] =>
+      specialize (Hn (midx, msg)
+                     (InMP_or_enqMP
+                        msgs (or_introl (conj eq_refl eq_refl))));
+      red in Hn; unfold map in Hn;
+      disc_caseDec Hn; auto
     end.
 
   Ltac solve_InvDirME_by_idx_false :=
@@ -307,7 +359,7 @@ Section InvDirME.
     end.
 
   Ltac solve_InvDirME_valid :=
-    split; [solve_InvDirME_NoRsI_by_silent
+    split; [solve_InvDirME_NoRsSI_by_silent
            |disc_getDir; solve_InvDirME_ObjInS_valid].
   
   Lemma mesi_InvDirME_step:
@@ -352,48 +404,46 @@ Section InvDirME.
 
         dest_in.
 
-        { disc_rule_conds_ex.
-          simpl_InvDirME_msgs.
-          disc_InvDirME.
-          solve_InvDirME_valid.
+        { disc_rule_conds_ex; disc_InvDirME.
+          { solve_InvDirME_valid. }
+          { solve_InvDirME_by_diff_dir. }
+          { destruct (idx_dec cidx oidx0); subst.
+            { solve_InvDirME_by_idx_false. }
+            { solve_InvDirME_valid. }
+          }
         }
         
-        { disc_rule_conds_ex; disc_InvDirME.
-          { solve_InvDirME_valid. }
+        { disc_rule_conds_ex; disc_InvDirME_pre.
+          { disc_NoRsME; solve_InvDirME_valid. }
           { disc_ObjDirME.
-            derive_child_idx_in oidx0.
-            solve_InvDirME_by_upRq_false oidx0.
+            solve_InvDirME_by_NoRsME_false.
           }
           { destruct (idx_dec cidx oidx0); subst.
             { solve_InvDirME_by_idx_false. }
-            { disc_InvDirME; solve_InvDirME_valid. }
+            { disc_NoRsME; solve_InvDirME_valid. }
           }
         }
 
         { disc_rule_conds_ex; simpl_InvDirME_msgs; disc_InvDirME.
-          { mred. }
-          { disc_ObjDirME; mred. }
+          disc_ObjDirME; mred.
         }
 
-        { disc_rule_conds_ex; disc_InvDirME.
-          { solve_InvDirME_valid. }
+        { disc_rule_conds_ex; disc_InvDirME_pre.
+          { disc_NoRsME; solve_InvDirME_valid. }
           { disc_ObjDirME.
-            derive_child_idx_in oidx0.
-            solve_InvDirME_by_upRq_false oidx0.
+            solve_InvDirME_by_NoRsME_false.
           }
           { destruct (idx_dec cidx oidx0); subst.
             { solve_InvDirME_by_idx_false. }
-            { disc_InvDirME; solve_InvDirME_valid. }
+            { disc_NoRsME; solve_InvDirME_valid. }
           }
         }
 
         { disc_rule_conds_ex; simpl_InvDirME_msgs; disc_InvDirME.
-          { mred. }
-          { disc_ObjDirME; mred. }
+          disc_ObjDirME; mred.
         }
         { disc_rule_conds_ex; simpl_InvDirME_msgs; disc_InvDirME.
-          { mred. }
-          { disc_ObjDirME; mred. }
+          disc_ObjDirME; mred.
         }
 
         { disc_rule_conds_ex; disc_InvDirME.
@@ -469,28 +519,37 @@ Section InvDirME.
 
       dest_in.
 
-      { disc_rule_conds_ex; simpl_InvDirME_msgs; disc_InvDirME.
-        { mred; disc_InvDirME.
-          solve_InvDirME_valid.
-        }
+      { disc_rule_conds_ex.
+        disc_MesiDownLockInv oidx Hmdl.
+        disc_InvDirME.
+        { solve_InvDirME_valid. }
         { solve_InvDirME_by_diff_dir. }
+        { destruct (idx_dec x oidx0); subst.
+          { solve_InvDirME_by_idx_false. }
+          { solve_InvDirME_valid. }
+        }
       }
 
       { disc_rule_conds_ex.
         disc_MesiDownLockInv oidx Hmdl.
-        simpl_InvDirME_msgs.
-        disc_InvDirME.
-        { mred; disc_InvDirME.
+        disc_InvDirME_pre.
+        { disc_NoRsME.
+          apply MsgsP_other_msg_id_deqMsgs_inv in H21;
+            [|apply H8|assumption|admit].
+          disc_NoRsME.
           solve_InvDirME_valid.
         }
-        { exfalso.
-          disc_ObjDirME.
-
-          derive_child_idx_in oidx0.
-          disc_MsgConflictsInv oidx0.
-          move H26 at bottom.
-          specialize (H26 ltac:(red; mred; simpl; eauto)); dest.
-          eapply H30; eauto.
+        { disc_ObjDirME.
+          solve_InvDirME_by_NoRsME_false.
+        }
+        { destruct (idx_dec x oidx0); subst.
+          { solve_InvDirME_by_idx_false. }
+          { disc_NoRsME.
+            apply MsgsP_other_msg_id_deqMsgs_inv in H23;
+              [|apply H8|assumption|admit].
+            disc_NoRsME.
+            solve_InvDirME_valid.
+          }
         }
       }
 
@@ -737,838 +796,6 @@ Section InvDirME.
 
 End InvDirME.
 
-Definition InvWBLocal (st: MState): Prop :=
-  forall oidx,
-    ost <+- (bst_oss st)@[oidx];
-      orq <+- (bst_orqs st)@[oidx];
-      (NoDowns oidx (bst_orqs st) (bst_msgs st) ->
-       (ost#[dir].(dir_st) <= mesiS \/ ObjInvWRq oidx (bst_msgs st)) ->
-       mesiS <= ost#[status]).
-
-Section InvWBLocal.
-  Variable (tr: tree).
-  Hypothesis (Htr: tr <> Node nil).
-
-  Let topo: DTree := fst (tree2Topo tr 0).
-  Let cifc: CIfc := snd (tree2Topo tr 0).
-  Let impl: System := impl Htr.
-
-  Lemma mesi_InvWBLocal_init:
-    Invariant.InvInit impl InvWBLocal.
-  Proof.
-    do 2 (red; simpl); intros.
-    destruct (implOStatesInit tr)@[oidx] as [ost|] eqn:Host; simpl; auto.
-    destruct (implORqsInit tr)@[oidx] as [orq|] eqn:Horq; simpl; auto.
-    intros; exfalso.
-    
-    red in H0; dest.
-    destruct (in_dec idx_dec pidx (c_li_indices cifc ++ c_l1_indices cifc)).
-    - subst cifc; rewrite c_li_indices_head_rootOf in i by assumption.
-      inv i.
-      + rewrite implOStatesInit_value_root in Hpost by assumption.
-        inv Hpost.
-        simpl in *; solve_mesi.
-      + rewrite implOStatesInit_value_non_root in Hpost by assumption.
-        inv Hpost.
-        simpl in *; solve_mesi.
-    - rewrite implOStatesInit_None in Hpost by assumption.
-      discriminate.
-  Qed.
-
-  Lemma mesi_InvWBLocal_ext_in:
-    forall oss orqs msgs,
-      InvWBLocal topo {| bst_oss := oss; bst_orqs := orqs; bst_msgs := msgs |} ->
-      InObjInds tr 0 {| bst_oss := oss; bst_orqs := orqs; bst_msgs := msgs |} ->
-      forall eins,
-        ValidMsgsExtIn impl eins ->
-        InvWBLocal topo {| bst_oss := oss; bst_orqs := orqs; bst_msgs := enqMsgs eins msgs |}.
-  Proof.
-    red; simpl; intros.
-    specialize (H _ _ H2); simpl in H.
-    destruct (oss@[oidx]) as [ost|] eqn:Host; simpl in *; auto.
-    destruct (orqs@[oidx]) as [orq|] eqn:Horq; simpl in *; auto.
-    destruct (oss@[pidx]) as [post|] eqn:Hpost; simpl in *; auto.
-    destruct (orqs@[pidx]) as [porq|] eqn:Hporq; simpl in *; auto.
-    intros; specialize (H H3); dest.
-    split; [assumption|intros].
-    destruct H5 as [idm [? ?]].
-    apply InMP_enqMsgs_or in H5.
-    destruct H5; [|apply H4; auto; do 2 red; eauto].
-    apply in_map with (f:= idOf) in H5; simpl in H5.
-    apply H1 in H5; simpl in H5.
-    exfalso; eapply DisjList_In_1.
-    - apply tree2Topo_minds_merqs_disj.
-    - eassumption.
-    - eapply tree2Topo_obj_chns_minds_SubList.
-      + specialize (H0 oidx); simpl in H0.
-        rewrite Host in H0; simpl in H0.
-        eassumption.
-      + destruct idm as [midx msg]; inv H6.
-        simpl; tauto.
-  Qed.
-
-  Lemma mesi_InvWBLocal_ext_out:
-    forall oss orqs msgs,
-      InvWBLocal topo {| bst_oss := oss; bst_orqs := orqs; bst_msgs := msgs |} ->
-      InObjInds tr 0 {| bst_oss := oss; bst_orqs := orqs; bst_msgs := msgs |} ->
-      forall (eouts: list (Id Msg)),
-        InvWBLocal topo {| bst_oss := oss;
-                      bst_orqs := orqs;
-                      bst_msgs := deqMsgs (idsOf eouts) msgs |}.
-  Proof.
-    red; simpl; intros.
-    specialize (H _ _ H1); simpl in H.
-    destruct (oss@[oidx]) as [ost|] eqn:Host; simpl in *; auto.
-    destruct (orqs@[oidx]) as [orq|] eqn:Horq; simpl in *; auto.
-    destruct (oss@[pidx]) as [post|] eqn:Hpost; simpl in *; auto.
-    destruct (orqs@[pidx]) as [porq|] eqn:Hporq; simpl in *; auto.
-    intros; specialize (H H2); dest.
-    split; [assumption|intros].
-    destruct H4 as [idm [? ?]].
-    apply InMP_deqMsgs in H4.
-    apply H3; auto.
-    do 2 red; eauto.
-  Qed.
-
-  Lemma InvWBLocal_other_msg_id_enqMP:
-    forall oss orqs msgs,
-      InvWBLocal topo {| bst_oss:= oss; bst_orqs:= orqs; bst_msgs:= msgs |} ->
-      forall midx msg,
-        msg.(msg_id) <> mesiInvWRq ->
-        InvWBLocal topo {| bst_oss:= oss; bst_orqs:= orqs;
-                      bst_msgs:= enqMP midx msg msgs |}.
-  Proof.
-    unfold InvWBLocal; simpl; intros.
-    specialize (H _ _ H1).
-    destruct (oss@[oidx]) as [ost|] eqn:Host; simpl in *; auto.
-    destruct (orqs@[oidx]) as [orq|] eqn:Horq; simpl in *; auto.
-    destruct (oss@[pidx]) as [post|] eqn:Hpost; simpl in *; auto.
-    destruct (orqs@[pidx]) as [porq|] eqn:Hporq; simpl in *; auto.
-    intros; specialize (H H2); dest.
-    split; [assumption|intros].
-    apply H3; auto.
-    destruct H4 as [idm [? ?]].
-    apply InMP_enqMP_or in H4; destruct H4.
-    - dest; subst.
-      exfalso; inv H5; auto.
-    - do 2 red; eauto.
-  Qed.
-  
-  Lemma InvWBLocal_other_msg_id_enqMsgs:
-    forall oss orqs msgs,
-      InvWBLocal topo {| bst_oss:= oss; bst_orqs:= orqs; bst_msgs:= msgs |} ->
-      forall nmsgs,
-        Forall (fun idm => (valOf idm).(msg_id) <> mesiInvWRq) nmsgs ->
-        InvWBLocal topo {| bst_oss:= oss; bst_orqs:= orqs;
-                      bst_msgs:= enqMsgs nmsgs msgs |}.
-  Proof.
-    intros.
-    generalize dependent msgs.
-    induction nmsgs as [|[nmidx nmsg] nmsgs]; simpl; intros; auto.
-    inv H0; dest.
-    apply IHnmsgs; auto.
-    apply InvWBLocal_other_msg_id_enqMP; assumption.
-  Qed.
-
-  Lemma InvWBLocal_deqMP:
-    forall oss orqs msgs,
-      InvWBLocal topo {| bst_oss:= oss; bst_orqs:= orqs; bst_msgs:= msgs |} ->
-      forall midx,
-        InvWBLocal topo {| bst_oss:= oss; bst_orqs:= orqs;
-                      bst_msgs:= deqMP midx msgs |}.
-  Proof.
-    unfold InvWBLocal; simpl; intros.
-    specialize (H _ _ H0).
-    destruct (oss@[oidx]) as [ost|] eqn:Host; simpl in *; auto.
-    destruct (orqs@[oidx]) as [orq|] eqn:Horq; simpl in *; auto.
-    destruct (oss@[pidx]) as [post|] eqn:Hpost; simpl in *; auto.
-    destruct (orqs@[pidx]) as [porq|] eqn:Hporq; simpl in *; auto.
-    intros; specialize (H H1); dest.
-    split; [assumption|intros].
-    destruct H3 as [idm [? ?]].
-    apply InMP_deqMP in H3.
-    apply H2; do 2 red; eauto.
-  Qed.
-
-  Lemma InvWBLocal_deqMsgs:
-    forall oss orqs msgs,
-      InvWBLocal topo {| bst_oss:= oss; bst_orqs:= orqs; bst_msgs:= msgs |} ->
-      forall minds,
-        InvWBLocal topo {| bst_oss:= oss; bst_orqs:= orqs;
-                      bst_msgs:= deqMsgs minds msgs |}.
-  Proof.
-    unfold InvWBLocal; simpl; intros.
-    specialize (H _ _ H0).
-    destruct (oss@[oidx]) as [ost|] eqn:Host; simpl in *; auto.
-    destruct (orqs@[oidx]) as [orq|] eqn:Horq; simpl in *; auto.
-    destruct (oss@[pidx]) as [post|] eqn:Hpost; simpl in *; auto.
-    destruct (orqs@[pidx]) as [porq|] eqn:Hporq; simpl in *; auto.
-    intros; specialize (H H1); dest.
-    split; [assumption|intros].
-    destruct H3 as [idm [? ?]].
-    apply InMP_deqMsgs in H3.
-    apply H2; do 2 red; eauto.
-  Qed.
-
-  Ltac simpl_InvWBLocal_msgs_enqMP :=
-    simpl;
-    try match goal with
-        | [H: msg_id ?rmsg = _ |- msg_id ?rmsg <> _] => rewrite H
-        end;
-    discriminate.
-
-  Ltac simpl_InvWBLocal_msgs_enqMsgs :=
-    let idm := fresh "idm" in
-    let Hin := fresh "H" in
-    apply Forall_forall; intros idm Hin;
-    apply in_map_iff in Hin; dest; subst;
-    simpl_InvWBLocal_msgs_enqMP.
-
-  Ltac simpl_InvWBLocal_msgs :=
-    repeat
-      (first [apply InvWBLocal_other_msg_id_enqMP; [|simpl_InvWBLocal_msgs_enqMP..]
-             |apply InvWBLocal_other_msg_id_enqMsgs; [|simpl_InvWBLocal_msgs_enqMsgs]
-             |apply InvWBLocal_deqMP
-             |apply InvWBLocal_deqMsgs
-             |assumption]).
-
-  Ltac disc_bind_true :=
-    repeat
-      match goal with
-      | |- _ <+- ?ov; _ =>
-        first [match goal with
-               | [H: ov = _ |- _] => rewrite H in *; simpl in *
-               end
-              |let Hov := fresh "H" in
-               let v := fresh "v" in
-               destruct ov as [v|] eqn:Hov; simpl in *; [|auto]]
-      end.
-
-  Ltac disc_InvWBLocal :=
-    repeat
-      match goal with
-      | [Hi: InvWBLocal _ _ |- InvWBLocal _ _] =>
-        let Hp := fresh "H" in
-        red; simpl; intros ? ? Hp;
-        specialize (Hi _ _ Hp); simpl in Hi;
-        mred; simpl;
-        try (exfalso; eapply parentIdxOf_not_eq; subst topo; eauto; fail)
-      | |- _ <+- _; _ => disc_bind_true
-      end.
-
-  Ltac solve_InvWBLocal_by_NoRqI :=
-    intros;
-    repeat
-      match goal with
-      | [Hn: NoRqI ?oidx ?msgs, Hi: ObjInvWRq ?oidx ?msgs |- _] =>
-        exfalso; eapply MsgExistsSig_MsgsNotExist_false;
-        [eassumption| |eassumption]; simpl; tauto
-      | [Hn: NoRqI ?oidx ?msgs, Hi: ObjInvRq ?oidx ?msgs |- _] =>
-        exfalso; eapply MsgExistsSig_MsgsNotExist_false;
-        [eassumption| |eassumption]; simpl; tauto
-      end.
-
-  Ltac solve_InvWBLocal_by_downlock :=
-    intros;
-    repeat
-      match goal with
-      | [Hn: ObjDirME _ _ _ |- _] => red in Hn; dest; mred; fail
-      | [Hn: ObjDirE _ _ _ |- _] => red in Hn; dest; mred; fail
-      end.
-
-  Ltac solve_InvWBLocal_by_diff_dir :=
-    intros;
-    match goal with
-    | [Hn: ObjDirME _ _ _ |- _] =>
-      red in Hn; dest; simpl in *; solve_mesi
-    | [Hn: ObjDirE _ _ _ |- _] =>
-      red in Hn; dest; simpl in *; solve_mesi
-    end.
-
-  Ltac solve_InvWBLocal_by_silent :=
-    intros;
-    match goal with
-    | [H: _ -> _ -> ObjOwned _ |- _] => apply H; try assumption
-    end;
-    repeat
-      match goal with
-      | [Hd: ObjDirME _ _ _ |- ObjDirME _ _ _] =>
-        red in Hd; dest; simpl in *;
-        red; simpl; repeat split; solve [assumption|mred]
-      | [Hd: ObjDirE _ _ _ |- ObjDirE _ _ _] =>
-        red in Hd; dest; simpl in *;
-        red; simpl; repeat split; solve [assumption|mred]
-      end.
-
-  Lemma mesi_InvWBLocal_step:
-    Invariant.InvStep impl step_m (InvWBLocal topo).
-  Proof. (* SKIP_PROOF_ON
-    red; intros.
-    pose proof (footprints_ok
-                  (mesi_GoodORqsInit Htr)
-                  (mesi_GoodRqRsSys Htr) H) as Hftinv.
-    pose proof (mesi_InObjInds H) as Hioi.
-    pose proof (mesi_MsgConflictsInv
-                  (@mesi_RootChnInv_ok _ Htr) H) as Hpmcf.
-    pose proof (mesi_MsgConflictsInv
-                  (@mesi_RootChnInv_ok _ Htr)
-                  (reachable_steps H (steps_singleton H1))) as Hnmcf.
-    pose proof (MesiDownLockInv_ok H) as Hmdl.
-    pose proof (mesi_InvWBLocalDir_ok H) as Hidir.
-    inv H1; [assumption
-            |apply mesi_InvWBLocal_ext_in; auto
-            |apply mesi_InvWBLocal_ext_out; auto
-            |].
-
-    simpl in H2; destruct H2; [subst|apply in_app_or in H1; destruct H1].
-    
-    - (*! Cases for the main memory *)
-
-      (** Abstract the root. *)
-      assert (In (rootOf (fst (tree2Topo tr 0)))
-                 (c_li_indices (snd (tree2Topo tr 0)))) as Hin.
-      { rewrite c_li_indices_head_rootOf by assumption.
-        left; reflexivity.
-      }
-
-      remember (rootOf (fst (tree2Topo tr 0))) as oidx; clear Heqoidx.
-
-      (** Do case analysis per a rule. *)
-      apply in_app_or in H3; destruct H3.
-
-      1: { (** Rules per a child *)
-        apply concat_In in H1; destruct H1 as [crls [? ?]].
-        apply in_map_iff in H1; destruct H1 as [cidx [? ?]]; subst.
-        dest_in.
-
-        { disc_rule_conds_ex.
-          simpl_InvWBLocal_msgs.
-          disc_InvWBLocal.
-          mred.
-        }
-
-        { disc_rule_conds_ex.
-          derive_child_idx_in cidx.
-          simpl_InvWBLocal_msgs.
-          disc_InvWBLocal.
-          { intros; split.
-            { intros; red; simpl.
-              destruct (fst (snd os)); intuition solve_mesi.
-            }
-            { assert (NoRqI oidx msgs)
-                by (solve_NoRqI_base; solve_NoRqI_by_no_locks oidx).
-              solve_InvWBLocal_by_NoRqI.
-            }
-          }
-          { intros.
-            red in H17; simpl in H17; dest; subst.
-            split.
-            {
-
-              Ltac derive_uplock_by_rqUp cidx :=
-                disc_MsgConflictsInv cidx;
-                (* TODO: must be in [disc_MsgConflictsInv]? *)
-                match goal with
-                | [Hcf: forall _ _, parentIdxOf _ cidx = Some _ -> _,
-                     Hp: parentIdxOf _ cidx = Some ?pidx,
-                     Ho: _@[?pidx] = Some _ |- _] =>
-                  specialize (Hcf _ _ Hp Ho); destruct Hcf
-                end;
-                match goal with
-                | [H: RqUpConflicts cidx _ _,
-                      Hr: FirstMPI _ (rqUpFrom cidx, ?rmsg) |- _] =>
-                  specialize (H (rqUpFrom cidx, rmsg) eq_refl (FirstMP_InMP Hr)); dest
-                end.
-
-                derive_uplock_by_rqUp oidx0.
-
-                destruct (v0@[upRq]); [intros; discriminate|exfalso; auto].
-            }
-            { assert (NoRqI oidx0 msgs)
-                by (solve_NoRqI_base; solve_NoRqI_by_rqUp oidx0).
-              solve_InvWBLocal_by_NoRqI.
-            }
-          }
-        }
-
-        { disc_rule_conds_ex.
-          simpl_InvWBLocal_msgs.
-          disc_InvWBLocal.
-          { mred. }
-          { solve_InvWBLocal_by_downlock. }
-        }
-
-        { disc_rule_conds_ex.
-          derive_child_idx_in cidx.
-          simpl_InvWBLocal_msgs.
-          disc_InvWBLocal.
-          { intros; split.
-            { intros; red; simpl.
-              destruct (fst (snd os)); intuition solve_mesi.
-            }
-            { assert (NoRqI oidx msgs)
-                by (solve_NoRqI_base; solve_NoRqI_by_no_locks oidx).
-              solve_InvWBLocal_by_NoRqI.
-            }
-          }
-          { intros.
-            red in H17; simpl in H17; dest; subst.
-            split.
-            { derive_uplock_by_rqUp oidx0.
-              destruct (v0@[upRq]); [intros; discriminate|exfalso; auto].
-            }
-            { assert (NoRqI oidx0 msgs)
-                by (solve_NoRqI_base; solve_NoRqI_by_rqUp oidx0).
-              solve_InvWBLocal_by_NoRqI.
-            }
-          }
-        }
-
-        { disc_rule_conds_ex.
-          simpl_InvWBLocal_msgs.
-          disc_InvWBLocal.
-          { mred. }
-          { solve_InvWBLocal_by_downlock. }
-        }
-
-        { disc_rule_conds_ex.
-          simpl_InvWBLocal_msgs.
-          disc_InvWBLocal.
-          { mred. }
-          { solve_InvWBLocal_by_downlock. }
-        }
-
-        { disc_rule_conds_ex.
-          simpl_InvWBLocal_msgs.
-          disc_InvWBLocal.
-          mred.
-        }
-
-        { disc_rule_conds_ex.
-          simpl_InvWBLocal_msgs.
-          disc_InvWBLocal.
-          { intros; split.
-            { intros.
-              admit.
-            }
-            { intros; apply H0; auto. }
-          }
-          { solve_InvWBLocal_by_diff_dir. }
-        }
-
-        { disc_rule_conds_ex.
-          simpl_InvWBLocal_msgs.
-          disc_InvWBLocal.
-          mred.
-        }
-
-        { disc_rule_conds_ex.
-          simpl_InvWBLocal_msgs.
-          disc_InvWBLocal.
-          { assert (NoRqI oidx msgs)
-              by (solve_NoRqI_base; solve_NoRqI_by_no_locks oidx).
-            solve_InvWBLocal_by_NoRqI.
-          }
-          { solve_InvWBLocal_by_diff_dir. }
-        }
-
-        { disc_rule_conds_ex.
-          simpl_InvWBLocal_msgs.
-          disc_InvWBLocal.
-        }
-
-        { disc_rule_conds_ex.
-          simpl_InvWBLocal_msgs.
-          disc_InvWBLocal.
-          solve_InvWBLocal_by_diff_dir.
-        }
-
-        { disc_rule_conds_ex.
-          simpl_InvWBLocal_msgs.
-          disc_InvWBLocal.
-        }
-
-        { disc_rule_conds_ex.
-          simpl_InvWBLocal_msgs.
-          disc_InvWBLocal.
-          { assert (NoRqI oidx msgs)
-              by (solve_NoRqI_base; solve_NoRqI_by_no_locks oidx).
-            solve_InvWBLocal_by_NoRqI.
-          }
-          { solve_InvWBLocal_by_diff_dir. }
-        }
-
-      }
-
-      dest_in.
-
-      { disc_rule_conds_ex.
-        simpl_InvWBLocal_msgs.
-        disc_InvWBLocal.
-        { disc_MesiDownLockInv oidx Hmdl.
-          intros; red in H0; dest; simpl in *; solve_mesi.
-        }
-        { solve_InvWBLocal_by_diff_dir. }
-      }
-
-      { disc_rule_conds_ex.
-        simpl_InvWBLocal_msgs.
-        disc_InvWBLocal.
-        { disc_MesiDownLockInv oidx Hmdl.
-          derive_InvWBLocalDir oidx.
-          intros; specialize (Hidir (or_introl H18)); simpl in *; solve_mesi.
-        }
-        { intros.
-          assert (NoRqI oidx0 msgs).
-          { solve_NoRqI_base.
-            (** TODO: need [solve_NoRqI_by_parent_lock] *)
-            all: admit.
-          }
-          solve_InvWBLocal_by_NoRqI.
-        }
-      }
-
-    - (*! Cases for Li caches *)
-
-      (** Derive some necessary information: each Li has a parent. *)
-      apply in_map_iff in H1; destruct H1 as [oidx [? ?]]; subst; simpl in *.
-
-      pose proof (tree2Topo_TreeTopoNode tr 0) as Htn.
-      pose proof (c_li_indices_tail_has_parent Htr _ _ H2).
-      destruct H1 as [pidx [? ?]].
-      pose proof (Htn _ _ H4); dest.
-      
-      (** Do case analysis per a rule. *)
-      apply in_app_or in H3; destruct H3.
-
-      1: { (** Rules per a child *)
-        apply concat_In in H3; destruct H3 as [crls [? ?]].
-        apply in_map_iff in H3; destruct H3 as [cidx [? ?]]; subst.
-        dest_in.
-
-        { disc_rule_conds_ex.
-          simpl_InvWBLocal_msgs.
-          disc_InvWBLocal.
-        }
-
-        { disc_rule_conds_ex.
-          derive_child_idx_in cidx.
-          simpl_InvWBLocal_msgs.
-          disc_InvWBLocal.
-          { assert (NoRqI oidx msgs)
-              by (solve_NoRqI_base; solve_NoRqI_by_no_locks oidx).
-            solve_InvWBLocal_by_NoRqI.
-          }
-          { intros.
-            red in H23; simpl in H23; dest; subst.
-            assert (NoRqI oidx0 msgs)
-              by (solve_NoRqI_base; solve_NoRqI_by_rqUp oidx0).
-            solve_InvWBLocal_by_NoRqI.
-          }
-        }
-
-        { disc_rule_conds_ex.
-          simpl_InvWBLocal_msgs.
-          disc_InvWBLocal.
-          solve_InvWBLocal_by_silent.
-        }
-
-        { disc_rule_conds_ex.
-          simpl_InvWBLocal_msgs.
-          disc_InvWBLocal.
-          solve_InvWBLocal_by_downlock.
-        }
-
-        { disc_rule_conds_ex.
-          simpl_InvWBLocal_msgs.
-          disc_InvWBLocal.
-          solve_InvWBLocal_by_silent.
-        }
-
-        { disc_rule_conds_ex.
-          derive_child_idx_in cidx.
-          simpl_InvWBLocal_msgs.
-          disc_InvWBLocal.
-          { assert (NoRqI oidx msgs)
-              by (solve_NoRqI_base; solve_NoRqI_by_no_locks oidx).
-            solve_InvWBLocal_by_NoRqI.
-          }
-          { intros.
-            red in H23; simpl in H23; dest; subst.
-            assert (NoRqI oidx0 msgs)
-              by (solve_NoRqI_base; solve_NoRqI_by_rqUp oidx0).
-            solve_InvWBLocal_by_NoRqI.
-          }
-        }
-
-        { disc_rule_conds_ex.
-          simpl_InvWBLocal_msgs.
-          disc_InvWBLocal.
-          solve_InvWBLocal_by_silent.
-        }
-
-        { disc_rule_conds_ex.
-          simpl_InvWBLocal_msgs.
-          disc_InvWBLocal.
-          solve_InvWBLocal_by_silent.
-        }
-
-        { disc_rule_conds_ex.
-          simpl_InvWBLocal_msgs.
-          disc_InvWBLocal.
-          solve_InvWBLocal_by_silent.
-        }
-
-        { disc_rule_conds_ex.
-          simpl_InvWBLocal_msgs.
-          disc_InvWBLocal.
-        }
-
-        { disc_rule_conds_ex.
-          simpl_InvWBLocal_msgs.
-          disc_InvWBLocal.
-          solve_InvWBLocal_by_diff_dir.
-        }
-
-        { disc_rule_conds_ex.
-          simpl_InvWBLocal_msgs.
-          disc_InvWBLocal.
-        }
-
-        { disc_rule_conds_ex.
-          simpl_InvWBLocal_msgs.
-          disc_InvWBLocal.
-          { assert (NoRqI oidx msgs)
-              by (solve_NoRqI_base; solve_NoRqI_by_no_locks oidx).
-            solve_InvWBLocal_by_NoRqI.
-          }
-          { solve_InvWBLocal_by_diff_dir. }
-        }
-
-        { disc_rule_conds_ex.
-          simpl_InvWBLocal_msgs.
-          disc_InvWBLocal.
-        }
-
-        { disc_rule_conds_ex.
-          simpl_InvWBLocal_msgs.
-          disc_InvWBLocal.
-          solve_InvWBLocal_by_diff_dir.
-        }
-
-        { disc_rule_conds_ex.
-          simpl_InvWBLocal_msgs.
-          disc_InvWBLocal.
-        }
-
-        { disc_rule_conds_ex.
-          simpl_InvWBLocal_msgs.
-          disc_InvWBLocal.
-          { assert (NoRqI oidx msgs)
-              by (solve_NoRqI_base; solve_NoRqI_by_no_locks oidx).
-            solve_InvWBLocal_by_NoRqI.
-          }
-          { solve_InvWBLocal_by_diff_dir. }
-        }
-
-      }
-
-      dest_in.
-
-      { disc_rule_conds_ex.
-        derive_footprint_info_basis oidx.
-        simpl_InvWBLocal_msgs.
-        disc_InvWBLocal.
-        { subst topo; disc_rule_conds_ex.
-          assert (NoRqI oidx msgs)
-            by (solve_NoRqI_base; solve_NoRqI_by_rsDown oidx).
-          solve_InvWBLocal_by_NoRqI.
-        }
-        { solve_InvWBLocal_by_diff_dir. }
-      }
-
-      { disc_rule_conds_ex.
-        derive_footprint_info_basis oidx.
-        simpl_InvWBLocal_msgs.
-        disc_InvWBLocal.
-        { subst topo; disc_rule_conds_ex.
-          assert (NoRqI oidx msgs)
-            by (solve_NoRqI_base; solve_NoRqI_by_rsDown oidx).
-          solve_InvWBLocal_by_NoRqI.
-        }
-        { intros.
-          (** TODO: need [solve_NoRqI_by_parent_lock] *)
-          all: admit.
-        }
-      }
-
-      { disc_rule_conds_ex.
-        simpl_InvWBLocal_msgs.
-        disc_InvWBLocal.
-        { disc_MesiDownLockInv oidx Hmdl.
-          intros; red in H0; dest; simpl in *; solve_mesi.
-        }
-        { solve_InvWBLocal_by_diff_dir. }
-      }
-
-      { disc_rule_conds_ex.
-        simpl_InvWBLocal_msgs.
-        disc_InvWBLocal.
-        { disc_MesiDownLockInv oidx Hmdl.
-          derive_InvWBLocalDir oidx.
-          intros; specialize (Hidir (or_introl H25)); simpl in *; solve_mesi.
-        }
-        { intros.
-          assert (NoRqI oidx0 msgs).
-          { solve_NoRqI_base.
-            (** TODO: need [solve_NoRqI_by_parent_lock] *)
-            all: admit.
-          }
-          solve_InvWBLocal_by_NoRqI.
-        }
-      }
-
-      { disc_rule_conds_ex.
-        simpl_InvWBLocal_msgs.
-        disc_InvWBLocal.
-
-        Ltac derive_downlock_by_rqDown cidx :=
-          disc_MsgConflictsInv cidx;
-          (* TODO: must be in [disc_MsgConflictsInv]? *)
-          match goal with
-          | [Hcf: forall _ _, parentIdxOf _ cidx = Some _ -> _,
-               Hp: parentIdxOf _ cidx = Some ?pidx,
-               Ho: _@[?pidx] = Some _ |- _] =>
-            specialize (Hcf _ _ Hp Ho); destruct Hcf
-          end;
-          match goal with
-          | [H: RqDownConflicts cidx _ _,
-                Ht: msg_type ?rmsg = MRq,
-                    Hr: FirstMPI _ (downTo cidx, ?rmsg) |- _] =>
-            specialize (H (downTo cidx, rmsg) eq_refl Ht (FirstMP_InMP Hr)); dest
-          end.
-
-        subst topo; disc_rule_conds_ex.
-        intros; derive_downlock_by_rqDown oidx; solve_InvWBLocal_by_downlock.
-      }
-
-      { disc_rule_conds_ex.
-        simpl_InvWBLocal_msgs.
-        disc_InvWBLocal.
-        solve_InvWBLocal_by_downlock.
-      }
-
-      { disc_rule_conds_ex.
-        simpl_InvWBLocal_msgs.
-        disc_InvWBLocal.
-        solve_InvWBLocal_by_downlock.
-      }
-
-      { disc_rule_conds_ex.
-        simpl_InvWBLocal_msgs.
-        disc_InvWBLocal.
-        { (** TODO: need [derive_downlock_by_child_uplock] *)
-          all: admit.
-        }
-        { solve_InvWBLocal_by_diff_dir. }
-      }
-
-      { disc_rule_conds_ex.
-        derive_footprint_info_basis oidx.
-        simpl_InvWBLocal_msgs.
-        disc_InvWBLocal.
-        { assert (NoRqI oidx msgs)
-            by (solve_NoRqI_base; solve_NoRqI_by_rsDown oidx).
-          solve_InvWBLocal_by_NoRqI.
-        }
-        { (** TODO: need [solve_NoRqI_by_parent_lock] *)
-          all: admit.
-        }
-      }
-
-      { disc_rule_conds_ex.
-        derive_footprint_info_basis oidx.
-        simpl_InvWBLocal_msgs.
-        disc_InvWBLocal.
-        { assert (NoRqI oidx msgs)
-            by (solve_NoRqI_base; solve_NoRqI_by_rsDown oidx).
-          solve_InvWBLocal_by_NoRqI.
-        }
-        { solve_InvWBLocal_by_downlock. }
-      }
-
-      { disc_rule_conds_ex.
-        simpl_InvWBLocal_msgs.
-        disc_InvWBLocal.
-        { disc_MesiDownLockInv oidx Hmdl.
-          derive_InvWBLocalDir oidx.
-          intros; specialize (Hidir (or_introl H24)); simpl in *; solve_mesi.
-        }
-        { intros.
-          assert (NoRqI oidx0 msgs).
-          { solve_NoRqI_base.
-            (** TODO: need [solve_NoRqI_by_parent_lock] *)
-            all: admit.
-          }
-          solve_InvWBLocal_by_NoRqI.
-        }
-      }
-
-      { disc_rule_conds_ex.
-        simpl_InvWBLocal_msgs.
-        disc_InvWBLocal.
-        subst topo; disc_rule_conds_ex.
-        intros; derive_downlock_by_rqDown oidx; solve_InvWBLocal_by_downlock.
-      }
-
-      { disc_rule_conds_ex.
-        simpl_InvWBLocal_msgs.
-        disc_InvWBLocal.
-        solve_InvWBLocal_by_downlock.
-      }
-
-      { disc_rule_conds_ex.
-        simpl_InvWBLocal_msgs.
-        disc_InvWBLocal.
-        solve_InvWBLocal_by_downlock.
-      }
-
-      { disc_rule_conds_ex.
-        simpl_InvWBLocal_msgs.
-        disc_InvWBLocal.
-        { (** TODO: need [derive_downlock_by_child_uplock] *)
-          all: admit.
-        }
-        { solve_InvWBLocal_by_diff_dir. }
-      }
-
-      { (** [liInvRqUpUp] *)
-        admit.
-      }
-
-      all: admit.
-
-    - (*! Cases for L1 caches *)
-
-      (** Derive some necessary information: each Li has a parent. *)
-      apply in_map_iff in H1; destruct H1 as [oidx [? ?]]; subst.
-
-      pose proof (tree2Topo_TreeTopoNode tr 0) as Htn.
-      pose proof (c_l1_indices_has_parent Htr _ _ H2).
-      destruct H1 as [pidx [? ?]].
-      pose proof (Htn _ _ H4); dest.
-
-      (** Do case analysis per a rule. *)
-      dest_in.
-      all: admit.
-
-      END_SKIP_PROOF_ON *) admit.
-      
-  Admitted.
-
-End InvWBLocal.
-
-
 Definition InvWB (topo: DTree) (st: MState): Prop :=
   forall oidx pidx,
     parentIdxOf topo oidx = Some pidx ->
@@ -1577,7 +804,7 @@ Definition InvWB (topo: DTree) (st: MState): Prop :=
       post <+- (bst_oss st)@[pidx];
       porq <+- (bst_orqs st)@[pidx];
       (ObjDirME porq post oidx ->
-       (ost#[dir].(dir_st) <= mesiS \/ ObjInvWRq oidx (bst_msgs st)) ->
+       ObjInvWRq oidx (bst_msgs st) ->
        mesiS <= ost#[status]).
 
 
